language_formal/spark2014_semantics/spark2014_core_subset(non-nested)/checks_generator.v
@@ -10,20 +10,20 @@ Require Export language_flagged.
 
 Inductive compile2_flagged_exp: expression -> expression_x -> Prop :=
     | C2_Flagged_Literal: forall ast_num l checkflags,
-        gen_check_flags (E_Literal ast_num l) checkflags ->
+        gen_exp_check_flags (E_Literal ast_num l) checkflags ->
         compile2_flagged_exp (E_Literal ast_num l) (E_Literal_X ast_num l checkflags) 
     | C2_Flagged_Name: forall ast_num n checkflags n_flagged,
-        gen_check_flags (E_Name ast_num n) checkflags ->
+        gen_exp_check_flags (E_Name ast_num n) checkflags ->
         compile2_flagged_name n n_flagged ->
         compile2_flagged_exp (E_Name ast_num n) (E_Name_X ast_num n_flagged checkflags) 
     | C2_Flagged_Binary_Operation: forall ast_num op e1 e2 checkflags e1_flagged e2_flagged,
-        gen_check_flags (E_Binary_Operation ast_num op e1 e2) checkflags ->
+        gen_exp_check_flags (E_Binary_Operation ast_num op e1 e2) checkflags ->
         compile2_flagged_exp e1 e1_flagged ->
         compile2_flagged_exp e2 e2_flagged ->
         compile2_flagged_exp (E_Binary_Operation ast_num op e1 e2)
                              (E_Binary_Operation_X ast_num op e1_flagged e2_flagged checkflags)
     | C2_Flagged_Unary_Operation: forall ast_num op e checkflags e_flagged,
-        gen_check_flags (E_Unary_Operation ast_num op e) checkflags ->
+        gen_exp_check_flags (E_Unary_Operation ast_num op e) checkflags ->
         compile2_flagged_exp e e_flagged ->
         compile2_flagged_exp (E_Unary_Operation ast_num op e) 
                              (E_Unary_Operation_X ast_num op e_flagged checkflags)
@@ -138,6 +138,12 @@ Inductive compile2_flagged_aspect_specifications: list aspect_specification -> l
 
 
 Inductive compile2_flagged_declaration: declaration -> declaration_x -> Prop :=
+    | C2_Flagged_D_Null_Declaration: 
+        compile2_flagged_declaration D_Null_Declaration D_Null_Declaration_X
+    | C2_Flagged_D_Type_Declaration: forall t t_flagged ast_num,
+        compile2_flagged_type_declaration t t_flagged ->
+        compile2_flagged_declaration (D_Type_Declaration   ast_num t) 
+                                     (D_Type_Declaration_X ast_num t_flagged)
     | C2_Flagged_D_Object_Declaration: forall o o_flagged ast_num,
         compile2_flagged_object_declaration o o_flagged ->
         compile2_flagged_declaration (D_Object_Declaration   ast_num o)
@@ -146,28 +152,20 @@ Inductive compile2_flagged_declaration: declaration -> declaration_x -> Prop :=
         compile2_flagged_procedure_declaration p p_flagged ->
         compile2_flagged_declaration (D_Procedure_Declaration   ast_num p)
                                      (D_Procedure_Declaration_X ast_num p_flagged) 
-    | C2_Flagged_D_Type_Declaration: forall t t_flagged ast_num,
-        compile2_flagged_type_declaration t t_flagged ->
-        compile2_flagged_declaration (D_Type_Declaration   ast_num t) 
-                                     (D_Type_Declaration_X ast_num t_flagged)
+    | C2_Flagged_D_Seq_Declaration: forall d1 d1_flagged d2 d2_flagged ast_num,
+        compile2_flagged_declaration d1 d1_flagged ->
+        compile2_flagged_declaration d2 d2_flagged ->
+        compile2_flagged_declaration (D_Seq_Declaration ast_num d1 d2) (D_Seq_Declaration_X ast_num d1_flagged d2_flagged)
 
 with compile2_flagged_procedure_declaration: procedure_declaration -> procedure_declaration_x -> Prop :=
        | C2_Flagged_Procedure_Declaration: forall aspects aspects_flagged params params_flagged 
                                                   decls decls_flagged stmt stmt_flagged ast_num p,
            compile2_flagged_aspect_specifications aspects aspects_flagged ->
            compile2_flagged_parameter_specifications params params_flagged ->
-           compile2_flagged_declarations decls decls_flagged ->
+           compile2_flagged_declaration decls decls_flagged ->
            compile2_flagged_stmt stmt stmt_flagged ->
            compile2_flagged_procedure_declaration (mkprocedure_declaration   ast_num p params aspects decls stmt)
-                                                  (mkprocedure_declaration_x ast_num p params_flagged aspects_flagged decls_flagged stmt_flagged)
-
-with compile2_flagged_declarations: list declaration -> list declaration_x -> Prop :=
-       | C2_Flagged_Declarations_Null:
-           compile2_flagged_declarations nil nil 
-       | C2_Flagged_Declarations_List: forall d d_flagged ld ld_flagged,
-           compile2_flagged_declaration  d  d_flagged ->
-           compile2_flagged_declarations ld ld_flagged ->
-           compile2_flagged_declarations (d :: ld) (d_flagged :: ld_flagged).
+                                                  (mkprocedure_declaration_x ast_num p params_flagged aspects_flagged decls_flagged stmt_flagged).
 
 
 (*
@@ -178,13 +176,380 @@ Inductive compile2_flagged_subprogram: subprogram -> subprogram_x -> Prop :=
                                     (Global_Procedure_X ast_num p_flagged).
 *)
 
-Require Import X_SparkTactics.
+
+(* ***************************************************************
+                          Funtion Version
+   *************************************************************** *)
+
+(** * Translator Function To Insert Checks *)
+
+Function compile2_flagged_exp_f (e: expression): expression_x :=
+  match e with
+  | E_Literal ast_num l => 
+      let checkflags := gen_exp_check_flags_f (E_Literal ast_num l) in
+        (E_Literal_X ast_num l checkflags)
+  | E_Name ast_num n => 
+      let checkflags := gen_exp_check_flags_f (E_Name ast_num n) in
+      let n_flagged := compile2_flagged_name_f n in
+        (E_Name_X ast_num n_flagged checkflags)
+  | E_Binary_Operation ast_num op e1 e2 =>
+      let checkflags := gen_exp_check_flags_f (E_Binary_Operation ast_num op e1 e2) in
+      let e1_flagged := compile2_flagged_exp_f e1 in
+      let e2_flagged := compile2_flagged_exp_f e2 in
+        (E_Binary_Operation_X ast_num op e1_flagged e2_flagged checkflags)
+  | E_Unary_Operation ast_num op e => 
+      let checkflags := gen_exp_check_flags_f (E_Unary_Operation ast_num op e) in
+      let e_flagged := compile2_flagged_exp_f e in
+        (E_Unary_Operation_X ast_num op e_flagged checkflags)
+  end
+
+with compile2_flagged_name_f (n: name): name_x :=
+  match n with
+  | E_Identifier ast_num x =>
+      let checkflags := gen_name_check_flags_f (E_Identifier ast_num x) in
+        (E_Identifier_X ast_num x checkflags)
+  | E_Indexed_Component ast_num x_ast_num x e =>
+      let checkflags := gen_name_check_flags_f (E_Indexed_Component ast_num x_ast_num x e) in
+      let e_flagged := compile2_flagged_exp_f e in
+        (E_Indexed_Component_X ast_num x_ast_num x e_flagged checkflags)
+  | E_Selected_Component ast_num x_ast_num x f =>
+      let checkflags := gen_name_check_flags_f (E_Selected_Component ast_num x_ast_num x f) in
+        (E_Selected_Component_X ast_num x_ast_num x f checkflags)
+  end.
+
+Function compile2_flagged_exps_f (le: list expression): list expression_x :=
+  match le with
+  | nil => nil
+  | e :: le' => 
+      let e_flagged := compile2_flagged_exp_f e in
+      let le_flagged := compile2_flagged_exps_f le' in
+        (e_flagged :: le_flagged)
+  end.
+
+Function compile2_flagged_stmt_f (c: statement): statement_x :=
+  match c with
+  | S_Null => S_Null_X
+  | S_Assignment ast_num x e =>
+      let x_flagged := compile2_flagged_name_f x in
+      let e_flagged := compile2_flagged_exp_f  e in
+        (S_Assignment_X ast_num x_flagged e_flagged)
+  | S_If ast_num e c1 c2 =>
+      let e_flagged := compile2_flagged_exp_f e in
+      let c1_flagged := compile2_flagged_stmt_f c1 in
+      let c2_flagged := compile2_flagged_stmt_f c2 in
+        (S_If_X ast_num e_flagged c1_flagged c2_flagged)
+  | S_While_Loop ast_num e c =>
+      let e_flagged := compile2_flagged_exp_f e in
+      let c_flagged := compile2_flagged_stmt_f c in
+        (S_While_Loop_X ast_num e_flagged c_flagged)
+  | S_Procedure_Call ast_num p_ast_num p args =>
+      let args_flagged := compile2_flagged_exps_f args in
+        (S_Procedure_Call_X ast_num p_ast_num p args_flagged)
+  | S_Sequence ast_num c1 c2 =>
+      let c1_flagged := compile2_flagged_stmt_f c1 in
+      let c2_flagged := compile2_flagged_stmt_f c2 in
+        (S_Sequence_X ast_num c1_flagged c2_flagged)
+  end.
+
+Function compile2_flagged_type_declaration_f (t: type_declaration): type_declaration_x :=
+  match t with
+  | Array_Type_Declaration ast_num tn t l u => 
+      (Array_Type_Declaration_X ast_num tn t l u)
+  | Record_Type_Declaration ast_num tn fs =>
+      (Record_Type_Declaration_X ast_num tn fs)
+  end.
+
+Function compile2_flagged_object_declaration_f (o: object_declaration): object_declaration_x :=
+  match o with
+  | mkobject_declaration ast_num x t None =>
+      (mkobject_declaration_x ast_num x t None)
+  | mkobject_declaration ast_num x t (Some e) => 
+      let e_flagged := compile2_flagged_exp_f e in
+        (mkobject_declaration_x ast_num x t (Some e_flagged))
+  end.
+
+Function compile2_flagged_object_declarations_f (lo: list object_declaration): list object_declaration_x :=
+  match lo with
+  | nil => nil
+  | o :: lo' => 
+      let o_flagged := compile2_flagged_object_declaration_f o in
+      let lo_flagged := compile2_flagged_object_declarations_f lo' in
+        (o_flagged :: lo_flagged)
+  end.
+
+Function compile2_flagged_parameter_specification_f (param: parameter_specification): parameter_specification_x :=
+  match param with
+  | mkparameter_specification   ast_num x m t =>
+      (mkparameter_specification_x ast_num x m t)
+  end.
+
+Function compile2_flagged_parameter_specifications_f (lparam: list parameter_specification): list parameter_specification_x :=
+  match lparam with
+  | nil => nil
+  | param :: lparam' =>
+      let param_flagged := compile2_flagged_parameter_specification_f param in
+      let lparam_flagged := compile2_flagged_parameter_specifications_f lparam' in
+        (param_flagged :: lparam_flagged)
+  end.
+
+Function compile2_flagged_aspect_specification_f (a: aspect_specification): aspect_specification_x :=
+  match a with
+  | mkaspect_specification ast_num mk e =>
+      let e_flagged := compile2_flagged_exp_f e in
+        (mkaspect_specification_x ast_num mk e_flagged)
+  end.
+
+Function compile2_flagged_aspect_specifications_f (la: list aspect_specification): list aspect_specification_x :=
+  match la with
+  | nil => nil
+  | a :: la' =>
+      let a_flagged := compile2_flagged_aspect_specification_f a in
+      let la_flagged := compile2_flagged_aspect_specifications_f la' in
+        (a_flagged :: la_flagged)
+  end.
+
+
+Function compile2_flagged_declaration_f (d: declaration): declaration_x :=
+  match d with
+  | D_Null_Declaration => D_Null_Declaration_X
+  | D_Type_Declaration ast_num t =>
+      let t_flagged := compile2_flagged_type_declaration_f t in
+        (D_Type_Declaration_X ast_num t_flagged)
+  | D_Object_Declaration ast_num o =>
+      let o_flagged := compile2_flagged_object_declaration_f o in
+        (D_Object_Declaration_X ast_num o_flagged)
+  | D_Procedure_Declaration ast_num p =>
+      let p_flagged := compile2_flagged_procedure_declaration_f p in
+        (D_Procedure_Declaration_X ast_num p_flagged)
+  | D_Seq_Declaration ast_num d1 d2 =>
+      let d1_flagged := compile2_flagged_declaration_f d1 in
+      let d2_flagged := compile2_flagged_declaration_f d2 in
+        (D_Seq_Declaration_X ast_num d1_flagged d2_flagged)
+  end
+
+with compile2_flagged_procedure_declaration_f (p: procedure_declaration): procedure_declaration_x :=
+  match p with
+  | mkprocedure_declaration ast_num p params aspects decls stmt =>
+      let aspects_flagged := compile2_flagged_aspect_specifications_f aspects in
+      let params_flagged := compile2_flagged_parameter_specifications_f params in
+      let decls_flagged := compile2_flagged_declaration_f decls in
+      let stmt_flagged := compile2_flagged_stmt_f stmt in
+        (mkprocedure_declaration_x ast_num p params_flagged aspects_flagged decls_flagged stmt_flagged)
+  end.
+
+(*
+Function compile2_flagged_declaration_f1 (d: declaration): declaration_x :=
+  match d with
+  | D_Object_Declaration ast_num o =>
+      let o_flagged := compile2_flagged_object_declaration_f o in
+        (D_Object_Declaration_X ast_num o_flagged)
+  | D_Type_Declaration ast_num t =>
+      let t_flagged := compile2_flagged_type_declaration_f t in
+        (D_Type_Declaration_X ast_num t_flagged)
+  | D_Procedure_Declaration ast_num p =>
+      let p_flagged :=
+          match p with
+          | mkprocedure_declaration ast_num p params aspects decls stmt =>
+              let aspects_flagged := compile2_flagged_aspect_specifications_f aspects in
+              let params_flagged := compile2_flagged_parameter_specifications_f params in
+              let decls_flagged := compile2_flagged_declaration_f decls in
+              let stmt_flagged := compile2_flagged_stmt_f stmt in
+                (mkprocedure_declaration_x ast_num p params_flagged aspects_flagged decls_flagged stmt_flagged)
+          end in
+        (D_Procedure_Declaration_X ast_num p_flagged)
+  | D_Seq_Declaration ast_num d1 d2 =>
+      let d1_flagged := compile2_flagged_declaration_f d1 in
+      let d2_flagged := compile2_flagged_declaration_f d2 in
+        (D_Seq_Declaration_X ast_num d1_flagged d2_flagged)
+  end.
+*)
+
+
+(* ***************************************************************
+                 Semantics Equivalence Proof
+   *************************************************************** *)
+
+(** * Semantics Equivalence Proof For Translator *)
+
+Scheme expression_ind := Induction for expression Sort Prop 
+                         with name_ind := Induction for name Sort Prop.
+
+Lemma compile2_flagged_exp_f_correctness: forall e e',
+  compile2_flagged_exp_f e = e' ->
+    compile2_flagged_exp e e'.
+Proof.
+  apply (expression_ind
+    (fun e: expression => forall (e' : expression_x),
+      compile2_flagged_exp_f e = e' ->
+      compile2_flagged_exp e e')
+    (fun n: name => forall (n': name_x),
+      compile2_flagged_name_f n = n' ->
+      compile2_flagged_name n n')
+    ); smack;
+  [destruct l | | destruct b | destruct u | | | ];
+  repeat progress constructor; smack.
+Qed.
+
+Lemma compile2_flagged_name_f_correctness: forall e e',
+  compile2_flagged_name_f e = e' ->
+    compile2_flagged_name e e'.
+Proof.
+  intros.
+  destruct e; smack;
+  repeat progress constructor;
+  apply compile2_flagged_exp_f_correctness; auto.  
+Qed.
+
+Lemma compile2_flagged_exps_f_correctness: forall le le',
+  compile2_flagged_exps_f le = le' ->
+    compile2_flagged_exps le le'.
+Proof.
+  induction le; smack.
+- constructor.
+- constructor.
+  + apply compile2_flagged_exp_f_correctness; auto.
+  + auto.
+Qed.
+  
+Lemma compile2_flagged_stmt_f_correctness: forall c c',
+  compile2_flagged_stmt_f c = c' ->
+    compile2_flagged_stmt c c'.
+Proof.
+  induction c; smack.
+- constructor.
+- constructor;
+  [ apply compile2_flagged_name_f_correctness |
+    apply compile2_flagged_exp_f_correctness 
+  ]; auto.
+- constructor;
+  [ apply compile2_flagged_exp_f_correctness | | ];
+  smack.
+- constructor;
+  [ apply compile2_flagged_exp_f_correctness | ];
+  smack.
+- constructor;
+  apply compile2_flagged_exps_f_correctness; auto.
+- constructor; auto.
+Qed.
+
+Lemma compile2_flagged_type_declaration_f_correctness: forall t t',
+  compile2_flagged_type_declaration_f t = t' ->
+      compile2_flagged_type_declaration t t'.
+Proof.
+  destruct t; smack;
+  constructor.  
+Qed.
+
+Lemma compile2_flagged_object_declaration_f_correctness: forall o o',
+  compile2_flagged_object_declaration_f o = o' ->
+    compile2_flagged_object_declaration o o'.
+Proof.
+  intros. 
+  functional induction compile2_flagged_object_declaration_f o; smack;
+  constructor.
+  apply compile2_flagged_exp_f_correctness; auto.
+Qed.
+
+Lemma compile2_flagged_object_declarations_f_correctness: forall lo lo',
+  compile2_flagged_object_declarations_f lo = lo' ->
+    compile2_flagged_object_declarations lo lo'.
+Proof.
+  induction lo; smack; 
+  constructor; smack.
+  apply compile2_flagged_object_declaration_f_correctness; auto.   
+Qed.
+
+Lemma compile2_flagged_parameter_specification_f_correctness: forall param param',
+  compile2_flagged_parameter_specification_f param = param' ->
+    compile2_flagged_parameter_specification param param'.
+Proof.
+  smack;
+  destruct param;
+  constructor.  
+Qed.
+
+Lemma compile2_flagged_parameter_specifications_f_correctness: forall lparam lparam',
+  compile2_flagged_parameter_specifications_f lparam = lparam' ->
+    compile2_flagged_parameter_specifications lparam lparam'.
+Proof.
+  induction lparam; smack;
+  constructor; smack.
+  apply compile2_flagged_parameter_specification_f_correctness; auto.
+Qed.
+
+Lemma compile2_flagged_aspect_specification_f_correctness: forall a a',
+  compile2_flagged_aspect_specification_f a = a' ->
+    compile2_flagged_aspect_specification a a'.
+Proof.
+  smack;
+  destruct a; constructor.
+  apply compile2_flagged_exp_f_correctness; auto.
+Qed.
+
+Lemma compile2_flagged_aspect_specifications_f_correctness: forall la la',
+  compile2_flagged_aspect_specifications_f la = la' ->
+    compile2_flagged_aspect_specifications la la'.
+Proof.
+  induction la; smack;
+  constructor; smack.
+  apply compile2_flagged_aspect_specification_f_correctness; auto.
+Qed.
+
+
+Scheme declaration_ind := Induction for declaration Sort Prop 
+                          with procedure_declaration_ind := Induction for procedure_declaration Sort Prop.
+
+Lemma compile2_flagged_declaration_f_correctness: forall d d',
+  compile2_flagged_declaration_f d = d' ->
+    compile2_flagged_declaration d d'.
+Proof.
+  apply (declaration_ind
+    (fun d: declaration => forall (d' : declaration_x),
+      compile2_flagged_declaration_f d = d' ->
+      compile2_flagged_declaration d d')
+    (fun p: procedure_declaration => forall (p': procedure_declaration_x),
+      compile2_flagged_procedure_declaration_f p = p' ->
+      compile2_flagged_procedure_declaration p p')
+    ); smack.
+- constructor.
+- constructor.
+  apply compile2_flagged_type_declaration_f_correctness; auto.
+- constructor.
+  apply compile2_flagged_object_declaration_f_correctness; auto.
+- constructor;
+  smack.
+- constructor;
+  smack.
+- constructor.
+  apply compile2_flagged_aspect_specifications_f_correctness; auto.
+  apply compile2_flagged_parameter_specifications_f_correctness; auto.
+  smack.
+  apply compile2_flagged_stmt_f_correctness; auto.
+Qed.
+
+Lemma compile2_flagged_procedure_declaration_f_correctness: forall p p',
+  compile2_flagged_procedure_declaration_f p = p' ->
+    compile2_flagged_procedure_declaration p p'.
+Proof.
+  intros;
+  destruct p; smack;
+  constructor;
+  [ apply compile2_flagged_aspect_specifications_f_correctness |
+    apply compile2_flagged_parameter_specifications_f_correctness |
+    apply compile2_flagged_declaration_f_correctness |
+    apply compile2_flagged_stmt_f_correctness 
+  ]; auto.
+Qed.
+
 
 (** * Lemmas *)
+
+Require Import X_SparkTactics.
+
 Lemma procedure_components_rel: forall p p',
   compile2_flagged_procedure_declaration p p' ->
   compile2_flagged_parameter_specifications (procedure_parameter_profile p) (procedure_parameter_profile_x p') /\
-  compile2_flagged_declarations (procedure_declarative_part p) (procedure_declarative_part_x p') /\
+  compile2_flagged_declaration (procedure_declarative_part p) (procedure_declarative_part_x p') /\
   compile2_flagged_stmt (procedure_statements p) (procedure_statements_x p').
 Proof.
   intros.
