language_formal/spark2014_semantics/spark2014_core_subset(non-nested)/test2014.v
@@ -9,69 +9,27 @@ Library_Unit_XX 1
     (Global_Procedure_XX 3
       (mkprocedure_declaration_xx 4
         (* Procedure Name *)
-        ((*Test*) 1)
-        (* Procedure Contract *)
-        (nil)
+        ((*Factorial*) 1)
         (* Formal Parameters *)
         (
-        (mkparameter_specification_xx 5 ((*N*) 1) In Integer) :: 
-        (mkparameter_specification_xx 6 ((*M*) 2) Out Integer) :: nil) 
+        (mkparameter_specification_xx 5 ((*N*) 1) Integer In) :: 
+        (mkparameter_specification_xx 6 ((*M*) 2) Integer Out) :: nil) 
+        (* Procedure Contract *)
+        (nil)  
         (* Object Declarations *)
-        (
-        (D_Type_Declaration_XX 7 (Record_Type_Declaration_XX 8 ((*RecordT*) 1) ((((*X*) 3), Integer) :: nil))) :: 
-        (D_Type_Declaration_XX 10 (Array_Type_Declaration_XX 11 ((*ArrayT*) 2) ((*componentType*) Integer) ((*lowerBound*) 0) ((*upperBound*) 5))) :: 
-        (D_Procedure_Declaration_XX 12 (mkprocedure_declaration_xx 13
-          (* Procedure Name *)
-          ((*Increase*) 2)
-          (* Procedure Contract *)
-          (nil)
-          (* Formal Parameters *)
-          (
-          (mkparameter_specification_xx 14 ((*X*) 4) In Integer) :: 
-          (mkparameter_specification_xx 15 ((*Y*) 5) Out Integer) :: nil) 
-          (* Object Declarations *)
-          (nil)
-          (* Procedure Body *)
-            (S_Assignment_XX 16 (E_Identifier_XX 17 ((*Y*) 5) (**(nil)**)) (E_Binary_Operation_XX 18 Plus (E_Name_XX 19 (E_Identifier_XX 20 ((*X*) 4) (**(nil)**)) (**(nil)**)) (E_Literal_XX 21 (Integer_Literal 1) (**(nil)**)) (**(Do_Overflow_Check :: nil)**)))
-        )) :: 
-        (D_Object_Declaration_XX 22 (mkobject_declaration_xx 23 ((*R*) 6) (Aggregate ((*RecordT*) 1)) None)) :: 
-        (D_Object_Declaration_XX 24 (mkobject_declaration_xx 25 ((*A*) 7) (Aggregate ((*ArrayT*) 2)) None)) :: 
-        (D_Object_Declaration_XX 26 (mkobject_declaration_xx 27 ((*Result*) 8) Integer (Some ((E_Literal_XX 28 (Integer_Literal 1) (**(nil)**)))))) :: 
-        (D_Object_Declaration_XX 29 (mkobject_declaration_xx 30 ((*T*) 9) Integer (Some ((E_Name_XX 31 (E_Identifier_XX 32 ((*Result*) 8) (**(nil)**)) (**(nil)**)))))) :: 
-        (D_Object_Declaration_XX 33 (mkobject_declaration_xx 34 ((*T1*) 10) Integer None)) :: 
-        (D_Object_Declaration_XX 35 (mkobject_declaration_xx 36 ((*T2*) 11) Integer None)) :: nil)
+        ((D_Seq_Declaration_XX 7 
+      (D_Object_Declaration_XX 8 (mkobject_declaration_xx 9 ((*Result*) 3) Integer (Some ((E_Literal_XX 10 (Integer_Literal 1) (**(nil)**)))))) 
+      (D_Object_Declaration_XX 11 (mkobject_declaration_xx 12 ((*T*) 4) Integer None))))
         (* Procedure Body *)
-          (S_Sequence_XX 37
-          (S_Assignment_XX 38 (E_Selected_Component_XX 39 40 ((*R*) 6) ((*X*) 3) (**(nil)**)) (E_Literal_XX 43 (Integer_Literal 1) (**(nil)**))) 
-          (S_Sequence_XX 44
-          (S_Assignment_XX 45 (E_Indexed_Component_XX 46 47 ((*A*) 7) (E_Literal_XX 49 (Integer_Literal 0) (**(nil)**)) (**(nil)**)) (E_Literal_XX 50 (Integer_Literal 1) (**(nil)**))) 
-          (S_Sequence_XX 51
-          (S_Assignment_XX 52 (E_Identifier_XX 53 ((*T1*) 10) (**(nil)**)) (E_Binary_Operation_XX 54 Plus (E_Name_XX 55 (E_Selected_Component_XX 56 57 ((*R*) 6) ((*X*) 3) (**(nil)**)) (**(nil)**)) (E_Name_XX 60 (E_Identifier_XX 61 ((*N*) 1) (**(nil)**)) (**(nil)**)) (**(Do_Overflow_Check :: nil)**))) 
-          (S_Sequence_XX 62
-          (S_Assignment_XX 63 (E_Identifier_XX 64 ((*T2*) 11) (**(nil)**)) (E_Binary_Operation_XX 65 Plus (E_Name_XX 66 (E_Indexed_Component_XX 67 68 ((*A*) 7) (E_Literal_XX 70 (Integer_Literal 0) (**(nil)**)) (**(nil)**)) (**(nil)**)) (E_Name_XX 71 (E_Identifier_XX 72 ((*T1*) 10) (**(nil)**)) (**(nil)**)) (**(Do_Overflow_Check :: nil)**))) 
-          (S_Sequence_XX 73
-          (S_Assignment_XX 74 (E_Identifier_XX 75 ((*T*) 9) (**(nil)**)) (E_Name_XX 76 (E_Identifier_XX 77 ((*T2*) 11) (**(nil)**)) (**(nil)**))) 
-          (S_Sequence_XX 78
-          (S_Procedure_Call_XX 79 80 ((*Increase*) 2) 
-            ((E_Name_XX 81 (E_Identifier_XX 82 ((*T2*) 11) (**(nil)**)) (**(nil)**)) :: (E_Name_XX 83 (E_Identifier_XX 84 ((*T*) 9) (**(nil)**)) (**(nil)**)) :: nil)
+          (S_Sequence_XX 13
+          (S_Assignment_XX 14 (E_Identifier_XX 15 ((*T*) 4) (**(nil)**)) (E_Name_XX 16 (E_Identifier_XX 17 ((*N*) 1) (**(nil)**)) (**(nil)**))) 
+          (S_Sequence_XX 18
+          (S_While_Loop_XX 19 (E_Binary_Operation_XX 20 Greater_Than (E_Name_XX 21 (E_Identifier_XX 22 ((*T*) 4) (**(nil)**)) (**(nil)**)) (E_Literal_XX 23 (Integer_Literal 0) (**(nil)**)) (**(nil)**))
+            (S_Sequence_XX 24
+            (S_Assignment_XX 25 (E_Identifier_XX 26 ((*Result*) 3) (**(nil)**)) (E_Binary_Operation_XX 27 Multiply (E_Name_XX 28 (E_Identifier_XX 29 ((*Result*) 3) (**(nil)**)) (**(nil)**)) (E_Name_XX 30 (E_Identifier_XX 31 ((*T*) 4) (**(nil)**)) (**(nil)**)) (**(Do_Overflow_Check :: nil)**))) 
+            (S_Assignment_XX 32 (E_Identifier_XX 33 ((*T*) 4) (**(nil)**)) (E_Binary_Operation_XX 34 Minus (E_Name_XX 35 (E_Identifier_XX 36 ((*T*) 4) (**(nil)**)) (**(nil)**)) (E_Literal_XX 37 (Integer_Literal 1) (**(nil)**)) (**(Do_Overflow_Check :: nil)**))))
           ) 
-          (S_Sequence_XX 85
-          (S_If_XX 86 (E_Binary_Operation_XX 87 Greater_Than (E_Name_XX 88 (E_Identifier_XX 89 ((*T*) 9) (**(nil)**)) (**(nil)**)) (E_Literal_XX 90 (Integer_Literal 0) (**(nil)**)) (**(nil)**))
-            (S_Assignment_XX 91 (E_Identifier_XX 92 ((*T*) 9) (**(nil)**)) (E_Binary_Operation_XX 93 Plus (E_Name_XX 94 (E_Identifier_XX 95 ((*T*) 9) (**(nil)**)) (**(nil)**)) (E_Literal_XX 96 (Integer_Literal 1) (**(nil)**)) (**(Do_Overflow_Check :: nil)**)))
-            S_Null_XX
-          ) 
-          (S_Sequence_XX 97
-          (S_If_XX 98 (E_Binary_Operation_XX 99 Greater_Than (E_Name_XX 100 (E_Identifier_XX 101 ((*T*) 9) (**(nil)**)) (**(nil)**)) (E_Literal_XX 102 (Integer_Literal 1) (**(nil)**)) (**(nil)**))
-            (S_Assignment_XX 103 (E_Identifier_XX 104 ((*T*) 9) (**(nil)**)) (E_Binary_Operation_XX 105 Plus (E_Name_XX 106 (E_Identifier_XX 107 ((*T*) 9) (**(nil)**)) (**(nil)**)) (E_Literal_XX 108 (Integer_Literal 2) (**(nil)**)) (**(Do_Overflow_Check :: nil)**)))
-            (S_Assignment_XX 109 (E_Identifier_XX 110 ((*T*) 9) (**(nil)**)) (E_Binary_Operation_XX 111 Minus (E_Name_XX 112 (E_Identifier_XX 113 ((*T*) 9) (**(nil)**)) (**(nil)**)) (E_Literal_XX 114 (Integer_Literal 1) (**(nil)**)) (**(Do_Overflow_Check :: nil)**)))
-          ) 
-          (S_Sequence_XX 115
-          (S_While_Loop_XX 116 (E_Binary_Operation_XX 117 Greater_Than (E_Name_XX 118 (E_Identifier_XX 119 ((*T*) 9) (**(nil)**)) (**(nil)**)) (E_Literal_XX 120 (Integer_Literal 0) (**(nil)**)) (**(nil)**))
-            (S_Sequence_XX 121
-            (S_Assignment_XX 122 (E_Identifier_XX 123 ((*Result*) 8) (**(nil)**)) (E_Binary_Operation_XX 124 Divide (E_Binary_Operation_XX 125 Multiply (E_Name_XX 126 (E_Identifier_XX 127 ((*Result*) 8) (**(nil)**)) (**(nil)**)) (E_Name_XX 128 (E_Identifier_XX 129 ((*T*) 9) (**(nil)**)) (**(nil)**)) (**(Do_Overflow_Check :: nil)**)) (E_Name_XX 130 (E_Identifier_XX 131 ((*N*) 1) (**(nil)**)) (**(nil)**)) (**(Do_Division_Check :: Do_Overflow_Check :: nil)**))) 
-            (S_Assignment_XX 132 (E_Identifier_XX 133 ((*T*) 9) (**(nil)**)) (E_Binary_Operation_XX 134 Minus (E_Name_XX 135 (E_Identifier_XX 136 ((*T*) 9) (**(nil)**)) (**(nil)**)) (E_Literal_XX 137 (Integer_Literal 1) (**(nil)**)) (**(Do_Overflow_Check :: nil)**))))
-          ) 
-          (S_Assignment_XX 138 (E_Identifier_XX 139 ((*M*) 2) (**(nil)**)) (E_Name_XX 140 (E_Identifier_XX 141 ((*Result*) 8) (**(nil)**)) (**(nil)**))))))))))))
+          (S_Assignment_XX 38 (E_Identifier_XX 39 ((*M*) 2) (**(nil)**)) (E_Name_XX 40 (E_Identifier_XX 41 ((*Result*) 3) (**(nil)**)) (**(nil)**)))))
       )
     )
   )
