language_formal/spark2014_semantics/spark2014_core_subset(non-nested)/test2014_ast.v
@@ -9,69 +9,27 @@ Library_Unit 1
     (Global_Procedure 3
       (mkprocedure_declaration 4
         (* Procedure Name *)
-        ((*Test*) 1)
-        (* Procedure Contract *)
-        (nil)
+        ((*Factorial*) 1)
         (* Formal Parameters *)
         (
-        (mkparameter_specification 5 ((*N*) 1) In Integer) :: 
-        (mkparameter_specification 6 ((*M*) 2) Out Integer) :: nil) 
+        (mkparameter_specification 5 ((*N*) 1) Integer In) :: 
+        (mkparameter_specification 6 ((*M*) 2) Integer Out) :: nil) 
+        (* Procedure Contract *)
+        (nil)  
         (* Object Declarations *)
-        (
-        (D_Type_Declaration 7 (Record_Type_Declaration 8 ((*RecordT*) 1) ((((*X*) 3), Integer) :: nil))) :: 
-        (D_Type_Declaration 10 (Array_Type_Declaration 11 ((*ArrayT*) 2) ((*componentType*) Integer) ((*lowerBound*) 0) ((*upperBound*) 5))) :: 
-        (D_Procedure_Declaration 12 (mkprocedure_declaration 13
-          (* Procedure Name *)
-          ((*Increase*) 2)
-          (* Procedure Contract *)
-          (nil)
-          (* Formal Parameters *)
-          (
-          (mkparameter_specification 14 ((*X*) 4) In Integer) :: 
-          (mkparameter_specification 15 ((*Y*) 5) Out Integer) :: nil) 
-          (* Object Declarations *)
-          (nil)
-          (* Procedure Body *)
-            (S_Assignment 16 (E_Identifier 17 ((*Y*) 5) (**(nil)**)) (E_Binary_Operation 18 Plus (E_Name 19 (E_Identifier 20 ((*X*) 4) (**(nil)**)) (**(nil)**)) (E_Literal 21 (Integer_Literal 1) (**(nil)**)) (**(Do_Overflow_Check :: nil)**)))
-        )) :: 
-        (D_Object_Declaration 22 (mkobject_declaration 23 ((*R*) 6) (Aggregate ((*RecordT*) 1)) None)) :: 
-        (D_Object_Declaration 24 (mkobject_declaration 25 ((*A*) 7) (Aggregate ((*ArrayT*) 2)) None)) :: 
-        (D_Object_Declaration 26 (mkobject_declaration 27 ((*Result*) 8) Integer (Some ((E_Literal 28 (Integer_Literal 1) (**(nil)**)))))) :: 
-        (D_Object_Declaration 29 (mkobject_declaration 30 ((*T*) 9) Integer (Some ((E_Name 31 (E_Identifier 32 ((*Result*) 8) (**(nil)**)) (**(nil)**)))))) :: 
-        (D_Object_Declaration 33 (mkobject_declaration 34 ((*T1*) 10) Integer None)) :: 
-        (D_Object_Declaration 35 (mkobject_declaration 36 ((*T2*) 11) Integer None)) :: nil)
+        ((D_Seq_Declaration 7 
+      (D_Object_Declaration 8 (mkobject_declaration 9 ((*Result*) 3) Integer (Some ((E_Literal 10 (Integer_Literal 1) (**(nil)**)))))) 
+      (D_Object_Declaration 11 (mkobject_declaration 12 ((*T*) 4) Integer None))))
         (* Procedure Body *)
-          (S_Sequence 37
-          (S_Assignment 38 (E_Selected_Component 39 40 ((*R*) 6) ((*X*) 3) (**(nil)**)) (E_Literal 43 (Integer_Literal 1) (**(nil)**))) 
-          (S_Sequence 44
-          (S_Assignment 45 (E_Indexed_Component 46 47 ((*A*) 7) (E_Literal 49 (Integer_Literal 0) (**(nil)**)) (**(nil)**)) (E_Literal 50 (Integer_Literal 1) (**(nil)**))) 
-          (S_Sequence 51
-          (S_Assignment 52 (E_Identifier 53 ((*T1*) 10) (**(nil)**)) (E_Binary_Operation 54 Plus (E_Name 55 (E_Selected_Component 56 57 ((*R*) 6) ((*X*) 3) (**(nil)**)) (**(nil)**)) (E_Name 60 (E_Identifier 61 ((*N*) 1) (**(nil)**)) (**(nil)**)) (**(Do_Overflow_Check :: nil)**))) 
-          (S_Sequence 62
-          (S_Assignment 63 (E_Identifier 64 ((*T2*) 11) (**(nil)**)) (E_Binary_Operation 65 Plus (E_Name 66 (E_Indexed_Component 67 68 ((*A*) 7) (E_Literal 70 (Integer_Literal 0) (**(nil)**)) (**(nil)**)) (**(nil)**)) (E_Name 71 (E_Identifier 72 ((*T1*) 10) (**(nil)**)) (**(nil)**)) (**(Do_Overflow_Check :: nil)**))) 
-          (S_Sequence 73
-          (S_Assignment 74 (E_Identifier 75 ((*T*) 9) (**(nil)**)) (E_Name 76 (E_Identifier 77 ((*T2*) 11) (**(nil)**)) (**(nil)**))) 
-          (S_Sequence 78
-          (S_Procedure_Call 79 80 ((*Increase*) 2) 
-            ((E_Name 81 (E_Identifier 82 ((*T2*) 11) (**(nil)**)) (**(nil)**)) :: (E_Name 83 (E_Identifier 84 ((*T*) 9) (**(nil)**)) (**(nil)**)) :: nil)
+          (S_Sequence 13
+          (S_Assignment 14 (E_Identifier 15 ((*T*) 4) (**(nil)**)) (E_Name 16 (E_Identifier 17 ((*N*) 1) (**(nil)**)) (**(nil)**))) 
+          (S_Sequence 18
+          (S_While_Loop 19 (E_Binary_Operation 20 Greater_Than (E_Name 21 (E_Identifier 22 ((*T*) 4) (**(nil)**)) (**(nil)**)) (E_Literal 23 (Integer_Literal 0) (**(nil)**)) (**(nil)**))
+            (S_Sequence 24
+            (S_Assignment 25 (E_Identifier 26 ((*Result*) 3) (**(nil)**)) (E_Binary_Operation 27 Multiply (E_Name 28 (E_Identifier 29 ((*Result*) 3) (**(nil)**)) (**(nil)**)) (E_Name 30 (E_Identifier 31 ((*T*) 4) (**(nil)**)) (**(nil)**)) (**(Do_Overflow_Check :: nil)**))) 
+            (S_Assignment 32 (E_Identifier 33 ((*T*) 4) (**(nil)**)) (E_Binary_Operation 34 Minus (E_Name 35 (E_Identifier 36 ((*T*) 4) (**(nil)**)) (**(nil)**)) (E_Literal 37 (Integer_Literal 1) (**(nil)**)) (**(Do_Overflow_Check :: nil)**))))
           ) 
-          (S_Sequence 85
-          (S_If 86 (E_Binary_Operation 87 Greater_Than (E_Name 88 (E_Identifier 89 ((*T*) 9) (**(nil)**)) (**(nil)**)) (E_Literal 90 (Integer_Literal 0) (**(nil)**)) (**(nil)**))
-            (S_Assignment 91 (E_Identifier 92 ((*T*) 9) (**(nil)**)) (E_Binary_Operation 93 Plus (E_Name 94 (E_Identifier 95 ((*T*) 9) (**(nil)**)) (**(nil)**)) (E_Literal 96 (Integer_Literal 1) (**(nil)**)) (**(Do_Overflow_Check :: nil)**)))
-            S_Null
-          ) 
-          (S_Sequence 97
-          (S_If 98 (E_Binary_Operation 99 Greater_Than (E_Name 100 (E_Identifier 101 ((*T*) 9) (**(nil)**)) (**(nil)**)) (E_Literal 102 (Integer_Literal 1) (**(nil)**)) (**(nil)**))
-            (S_Assignment 103 (E_Identifier 104 ((*T*) 9) (**(nil)**)) (E_Binary_Operation 105 Plus (E_Name 106 (E_Identifier 107 ((*T*) 9) (**(nil)**)) (**(nil)**)) (E_Literal 108 (Integer_Literal 2) (**(nil)**)) (**(Do_Overflow_Check :: nil)**)))
-            (S_Assignment 109 (E_Identifier 110 ((*T*) 9) (**(nil)**)) (E_Binary_Operation 111 Minus (E_Name 112 (E_Identifier 113 ((*T*) 9) (**(nil)**)) (**(nil)**)) (E_Literal 114 (Integer_Literal 1) (**(nil)**)) (**(Do_Overflow_Check :: nil)**)))
-          ) 
-          (S_Sequence 115
-          (S_While_Loop 116 (E_Binary_Operation 117 Greater_Than (E_Name 118 (E_Identifier 119 ((*T*) 9) (**(nil)**)) (**(nil)**)) (E_Literal 120 (Integer_Literal 0) (**(nil)**)) (**(nil)**))
-            (S_Sequence 121
-            (S_Assignment 122 (E_Identifier 123 ((*Result*) 8) (**(nil)**)) (E_Binary_Operation 124 Divide (E_Binary_Operation 125 Multiply (E_Name 126 (E_Identifier 127 ((*Result*) 8) (**(nil)**)) (**(nil)**)) (E_Name 128 (E_Identifier 129 ((*T*) 9) (**(nil)**)) (**(nil)**)) (**(Do_Overflow_Check :: nil)**)) (E_Name 130 (E_Identifier 131 ((*N*) 1) (**(nil)**)) (**(nil)**)) (**(Do_Division_Check :: Do_Overflow_Check :: nil)**))) 
-            (S_Assignment 132 (E_Identifier 133 ((*T*) 9) (**(nil)**)) (E_Binary_Operation 134 Minus (E_Name 135 (E_Identifier 136 ((*T*) 9) (**(nil)**)) (**(nil)**)) (E_Literal 137 (Integer_Literal 1) (**(nil)**)) (**(Do_Overflow_Check :: nil)**))))
-          ) 
-          (S_Assignment 138 (E_Identifier 139 ((*M*) 2) (**(nil)**)) (E_Name 140 (E_Identifier 141 ((*Result*) 8) (**(nil)**)) (**(nil)**))))))))))))
+          (S_Assignment 38 (E_Identifier 39 ((*M*) 2) (**(nil)**)) (E_Name 40 (E_Identifier 41 ((*Result*) 3) (**(nil)**)) (**(nil)**)))))
       )
     )
   )
